dynamic ifc

examples/rel/DynamicIFC2.fst
@@ -7,6 +7,7 @@ open FStar.DM4F.LabeledIntStoreExcFixed
 
 module ISFR = FStar.DM4F.LabeledIntStoreFixedReader
 
+
 type binop =
 | Plus
 | Minus
@@ -42,20 +43,21 @@ type com =
 
 
 type label_fun = id -> Tot label
-irreducible let trigger_leq (h:rel heap) (x:id) = True 
 
-type env_eq (h : rel heap) = (forall (x:id). {:pattern (trigger_leq h x)} snd (sel (R?.l h) x) = snd (sel (R?.r h) x))
+let trigger_eq (h:rel heap) (x:id) = True
+
+type env_eq (h : rel heap) = (forall (x:id).  (* {:pattern (trigger_eq h x)} *) snd (sel (R?.l h) x) = snd (sel (R?.r h) x))
 
 type low_equiv (h:rel heap) =
-  (forall (x:id). {:pattern (trigger_leq h x)} (fun (vl,ll) (vr,lr) -> ll = Low ==> vl = vr)
+  (forall (x:id). (* {:pattern (trigger_eq h x)} *) (fun (vl,ll) (vr,lr) -> ll = Low ==> vl = vr)
       (index (R?.l h) x)  (index (R?.r h) x))
 
 type low_equiv_env (env:label_fun) (h1:rel heap) =
-  (forall (x:id). (* {:pattern (env x)} *) env x = Low ==> index (R?.l h1) x = index (R?.r h1) x)
+  (forall (x:id). env x = Low ==> index (R?.l h1) x = index (R?.r h1) x)
 
 
 type no_sensitive_upd (h:heap) (pc:label) (h':heap) =
-  forall (x:id). (* {:pattern (trigger_nsu x)} *) (fun (v,l) (v',l') -> 
+  forall (x:id). (fun (v,l) (v',l') -> 
     (l' <= l /\
     (l < pc ==> v = v') /\
     (l <= pc ==> l = l')))
@@ -163,12 +165,12 @@ let interpret_com (h0:heap) (c:com) (pc:label) : Tot (option heap)
   | None, _ -> None
 
 
+(*
 (* Some test cases *)
 
-  (*
 let h0 = upd (upd (create (5,Low)) (to_id 3) (5, High)) (to_id 4) (5, High)
 
-#set-options "--z3rlimit 30"
+#set-options "--z3rlimit 60 --max_fuel 16 --max_ifuel 16"
 (* l1 := h1 *)
 let p1 = Assign (to_id 1) (AVar (to_id 3))
 let test1 = assert_norm (None? (interpret_com h0 p1 Low))
@@ -181,7 +183,7 @@ let test2 = assert_norm (Some? (interpret_com h0 p2 Low))
 let p3 = If (AOp Plus (AVar (to_id 3)) (AInt 2)) (Assign (to_id 1) (AInt 0)) Skip
 let test3 = assert_norm (None? (interpret_com h0 p3 Low))
 
-(* This is example shows the weak semantic of the monitor's security *)
+(* This is example shows the "weak" semantic of the monitor's security *)
 (* If (h1 - 5  <> 0 then {l1 := 9}  [env0(h1) = 5] *)
 let p4 = If (AOp Plus (AVar (to_id 3)) (AInt (- 5))) (Assign (to_id 1) (AInt 0)) Skip
 let test4 = assert_norm (Some? (interpret_com h0 p4 Low))
@@ -208,21 +210,95 @@ val no_sens_upd_pc : unit ->
   Lemma (forall h h'. no_sensitive_upd h High h' ==> no_sensitive_upd h Low h')
 let no_sens_upd_pc () = () 
 
+type high_pc_type (c:com) (h:heap) (pc:label) = 
+  begin
+    let o = (interpret_com h c pc) in 
+    (Some? o ==> no_sensitive_upd h pc (Some?.v o))
+  end
 
-#set-options "--z3rlimit 10"
+#set-options "--z3rlimit 30 "
 val high_pc_assign : (x:id) -> (e:exp) -> (h:heap) -> (pc:label) ->
-  Lemma (
-      (let o = (interpret_com h (Assign x e) pc) in 
-      (Some? o ==> no_sensitive_upd h pc (Some?.v o))))
+  Lemma (high_pc_type (Assign x e) h pc)
 let high_pc_assign x e h pc = ()
+#reset-options
 
-#set-options "--z3rlimit 60 --initial_fuel 1 --max_fuel 1 "
+
+#set-options "--z3rlimit 500 --initial_fuel 1 --max_fuel 1"
+val high_pc_while : (e:exp) -> (body:com) -> (v:exp) -> (h:heap) -> (pc:label) -> 
+  Lemma 
+    (requires 
+      (
+      let c = While e body v in 
+      let v0,l  = interpret_exp h e in
+      if v0 <> 0 then
+      begin
+        let o = interpret_com h body (join l pc)in
+        if Some? o then
+        begin
+          let h' = Some?.v o in
+          high_pc_type body h (join l pc) /\
+          begin
+            let m0 = interpret_exp' h v in
+            let m1 = interpret_exp' h' v in
+            if m0 > m1 then
+            begin
+              let o2 = interpret_com h' c pc in
+              if Some? o2 then
+              begin
+                let h'' = Some?.v o2 in
+                high_pc_type c h' pc
+              end
+              else True
+            end
+            else True
+          end
+        end
+        else True
+      end
+      else True))
+    (ensures (high_pc_type (While e body v) h pc))
+let high_pc_while e body v h pc = 
+  let c = While e body v in
+  let r = interpret_com h c pc in
+  let v0,l  = interpret_exp h e in
+  if v0 <> 0 then
+  begin
+    let o = interpret_com h body (join l pc) in
+    if Some? o then
+    begin
+      let h' = Some?.v o in
+      cut (high_pc_type body h (join l pc));
+      let m0 = interpret_exp' h v in
+      let m1 = interpret_exp' h' v in
+      if m0 > m1 then
+      begin
+        let o2 = interpret_com h' c pc in
+        if Some? o2 then
+        begin
+          let h'' = Some?.v o2 in
+          cut (high_pc_type c h' pc);
+          cut (Some? r /\ Some?.v r = h'');
+          no_sens_trans (join l pc) pc h h' h''
+        end
+        else
+          cut(None? r)
+      end
+      else
+        cut(None? r)
+    end
+    else
+      cut(None? r)
+  end
+  else
+    cut (Some? r /\ Some?.v r = h)
+
+#reset-options
+    
+#set-options "--z3rlimit 1000 --initial_fuel 1 --max_fuel 1"
 val high_pc : (c:com) -> (h:heap) -> (pc:label) ->
   Lemma
     (requires True)
-    (ensures 
-      (let o = (interpret_com h c pc) in 
-      (Some? o ==> no_sensitive_upd h pc (Some?.v o))))
+    (ensures high_pc_type c h pc)
   (decreases %[c; decr_while h c])
 let rec high_pc c h pc =
   match c with
@@ -250,19 +326,15 @@ let rec high_pc c h pc =
         no_sens_trans pc pc h h' h''
       end
     end
-        (*
-    *)
-  | _ -> admit ()
-  (*
   | While e body v -> 
     let v0,l  = interpret_exp h e in
     if v0 <> 0 then
     begin
-      let o = interpret_com h body (join pc l)in
+      let o = interpret_com h body (join l pc)in
       if Some? o then
       begin
         let h' = Some?.v o in
-        high_pc body h (join pc l);
+        high_pc body h (join l pc);
         let m0 = interpret_exp' h v in
         let m1 = interpret_exp' h' v in
         if m0 > m1 then
@@ -270,25 +342,24 @@ let rec high_pc c h pc =
           let o2 = interpret_com h' c pc in
           if Some? o2 then
           begin
-            let h'' = Some?.v o2 in
-            high_pc c h' pc;
-            no_sens_trans (join pc l) pc h h' h''
+            high_pc c h' pc
           end
         end
       end
-    end
-    *)
+    end;
+    high_pc_while e body v h pc
+
 
 #reset-options
 
-#set-options "--z3rlimit 15"
+#set-options "--z3rlimit 15 "
 val dyn_ifc_exp : (e:exp) -> (h:(rel heap)) ->
     Lemma 
       (requires (low_equiv h /\ env_eq h))
-      (ensures ((fun (vl,ll)  (vr,lr) ->
-        lr = ll /\ (Low? lr ==> vl = vr))
-        (interpret_exp (R?.l h) e)
-        (interpret_exp (R?.r h) e)))
+      (ensures (
+        let vl,ll = interpret_exp (R?.l h) e in 
+        let vr,lr = interpret_exp (R?.r h) e in 
+          lr = ll /\ (Low? lr ==> vl = vr)))
 let rec dyn_ifc_exp e h  =
   match e with
   | AInt _ -> ()
@@ -296,41 +367,178 @@ let rec dyn_ifc_exp e h  =
   | AOp _ e1 e2 -> dyn_ifc_exp e1 h; dyn_ifc_exp e2 h
 
 
+
+type ifc_type (c:com) (pc:label) (h:rel heap) = 
+  begin
+    let ol = (interpret_com (R?.l h) c pc) in 
+     let or = (interpret_com (R?.r h) c pc) in 
+     if (Some? ol && Some? or) then
+     begin
+       let h' = R (Some?.v ol) (Some?.v or) in 
+       low_equiv h' /\ env_eq h'
+     end
+     else True
+  end
+
+
+#set-options "--z3rlimit 10 "
+val dyn_ifc_assign : (x:id) -> (e:exp) -> (pc:label) -> (h:rel heap) -> 
+  Lemma
+      (requires (low_equiv h /\ env_eq h))
+      (ensures (ifc_type (Assign x e) pc h))
+let dyn_ifc_assign x e pc h = dyn_ifc_exp e h 
 #reset-options
-#set-options "--z3rlimit 2000 --initial_fuel 1 --max_fuel 1"
+
+
+#set-options "--z3rlimit 500 --initial_fuel 1 --max_fuel 2 "
+val dyn_ifc_while : (e:exp) -> (body:com) -> (v:exp) -> (pc:label) -> (h:rel heap) -> 
+   Lemma
+      (requires (low_equiv h /\ env_eq h /\ 
+        begin
+          let R hl hr = h in 
+          let c = While e body v in 
+          let v0l,ll  = interpret_exp hl e in
+          let v0r,lr  = interpret_exp hr e in
+          match v0l <> 0, v0r <> 0 with
+          | true, true ->  
+            let ol = interpret_com hl body (join ll pc)in
+            let or = interpret_com hr body (join lr pc)in
+            if (Some? ol && Some? or) then
+            begin
+              ifc_type body (join ll pc) h /\ 
+              begin
+                let hl' = Some?.v ol in
+                let hr' = Some?.v or in
+                let m0l = interpret_exp' hl v in
+                let m1l = interpret_exp' hl' v in
+                let m0r = interpret_exp' hr v in
+                let m1r = interpret_exp' hr' v in
+                if m0l > m1l && m0r > m1r then
+                  ifc_type c pc (R hl' hr')
+                else True
+              end
+            end
+            else True
+          | true, false  ->
+            let ol = interpret_com hl body High in
+            if (Some? ol) then
+            begin
+              let hl' = Some?.v ol in
+              let m0l = interpret_exp' hl v in
+              let m1l = interpret_exp' hl' v in
+              if m0l > m1l then
+                ifc_type c pc (R hl' hr)
+              else True
+            end
+            else True
+          | false, true -> 
+            let or = interpret_com hr body High in
+            if (Some? or) then
+            begin
+              let hr' = Some?.v or in
+              let m0r = interpret_exp' hr v in
+              let m1r = interpret_exp' hr' v in
+              if m0r > m1r then
+                ifc_type c pc (R hl hr')
+              else True
+            end
+            else True
+          | false, false -> True
+        end))
+      (ensures (ifc_type (While e body v) pc h))
+let dyn_ifc_while e body v pc h =  
+  let R hl hr = h in 
+  let c = While e body v in 
+  let rl = interpret_com hl c pc in 
+  let rr = interpret_com hr c pc in 
+  let v0l,ll  = interpret_exp hl e in
+  let v0r,lr  = interpret_exp hr e in
+  dyn_ifc_exp e h;
+  match v0l <> 0, v0r <> 0 with
+  | true, true -> 
+      let ol = interpret_com hl body (join ll pc) in
+      let or = interpret_com hr body (join lr pc) in
+      if (Some? ol && Some? or) then
+      begin
+        begin
+          cut (ifc_type body (join ll pc) h);
+          let hl' = Some?.v ol in
+          let hr' = Some?.v or in
+          let m0l = interpret_exp' hl v in
+          let m1l = interpret_exp' hl' v in
+          let m0r = interpret_exp' hr v in
+          let m1r = interpret_exp' hr' v in
+          if m0l > m1l && m0r > m1r then
+          begin
+            cut (ifc_type c pc (R hl' hr'));
+            cut (rl = interpret_com hl' c pc);
+            cut (rr = interpret_com hr' c pc)
+          end
+        end
+      end
+  | true, false ->
+      cut (High? ll);
+      let ol = interpret_com hl body High in
+      if (Some? ol) then
+      begin
+        let hl' = Some?.v ol in
+        high_pc body hl High;
+        let m0l = interpret_exp' hl v in
+        let m1l = interpret_exp' hl' v in
+        if m0l > m1l then
+        begin 
+          cut (ifc_type c  pc (R hl' hr));
+          cut (rl = interpret_com hl' c pc)
+        end
+      end
+  | false, true -> 
+      cut (High? lr);
+      let or = interpret_com hr body High in
+      if (Some? or) then
+      begin
+        let hr' = Some?.v or in
+        high_pc body hr High;
+        let m0r = interpret_exp' hr v in
+        let m1r = interpret_exp' hr' v in
+        if m0r > m1r then
+        begin
+          cut (ifc_type c  pc (R hl hr'));
+          cut (rr = interpret_com hr' c pc)
+        end
+      end
+ | false, false -> ()
+
+#reset-options
+
+
+#set-options "--z3rlimit 1000 --initial_fuel 1 --max_fuel 1" 
 val dyn_ifc' : (c:com) -> (pc:label) -> (h:(rel heap)) ->
     Lemma
       (requires (low_equiv h /\ env_eq h))
-      (ensures ((fun r1 r2 -> (Some? r1 /\ Some? r2) ==>
-        (fun hl hr ->
-          (low_equiv (R hl hr) /\
-           env_eq (R hl hr)))
-        (Some?.v r1) (Some?.v r2))
-      (interpret_com (R?.l h) c pc)
-      (interpret_com (R?.r h) c pc)))
-      (decreases %[c; decr_while (R?.l h) c; decr_while (R?.r h) c])
+      (ensures (ifc_type c pc h))
+      (decreases %[c; decr_while (R?.l h) c + decr_while (R?.r h) c])
 let rec dyn_ifc' c pc h  =
   let (R hl hr) = h in
   if Low? pc then
   begin
     match c with
     | Skip -> ()
-    | Assign x e -> admit () //dyn_ifc_exp e h
+    | Assign x e -> dyn_ifc_assign x e pc h
     | If e ct cf ->
         dyn_ifc_exp e h;
         (match interpret_exp hl e, interpret_exp hr e with
         | (0, ll) , (0, lr) ->
-            dyn_ifc' cf (join pc ll) h
+            dyn_ifc' cf (join ll pc) h
         | (0, ll) , (_, lr) ->
             cut (High? ll);
             high_pc cf hl High;
-            high_pc ct hr High; ()
+            high_pc ct hr High 
         | (_, ll) , (0, lr) ->
             cut (High? ll);
             high_pc ct hl High;
-            high_pc cf hr High; ()
+            high_pc cf hr High
         | (_, ll) , (_, lr) ->
-            dyn_ifc' ct (join pc ll) h)
+            dyn_ifc' ct (join ll pc) h)
     | Seq c1 c2 -> 
         let ol = interpret_com hl c1 pc in
         let or = interpret_com hr c1 pc in
@@ -346,16 +554,14 @@ let rec dyn_ifc' c pc h  =
       let v0l,ll  = interpret_exp hl e in
       let v0r,lr  = interpret_exp hr e in
       (match v0l <> 0, v0r <> 0 with
-      | true, true ->
-        let ol = interpret_com hl body (join pc ll)in
-        let or = interpret_com hr body (join pc lr)in
+      | true, true ->  
+        let ol = interpret_com hl body (join ll pc)in
+        let or = interpret_com hr body (join lr pc)in
         if (Some? ol && Some? or) then
         begin
           dyn_ifc' body (join ll pc) h;
           let hl' = Some?.v ol in
           let hr' = Some?.v or in
-          high_pc body hl(join ll pc) ;
-          high_pc body hr(join lr pc) ;
           let m0l = interpret_exp' hl v in
           let m1l = interpret_exp' hl' v in
           let m0r = interpret_exp' hr v in
@@ -364,7 +570,6 @@ let rec dyn_ifc' c pc h  =
             dyn_ifc' c pc (R hl' hr')
         end
       | true, false  ->
-        cut (High? ll);
         let ol = interpret_com hl body High in
         if (Some? ol) then
         begin
@@ -373,10 +578,12 @@ let rec dyn_ifc' c pc h  =
           let m0l = interpret_exp' hl v in
           let m1l = interpret_exp' hl' v in
           if m0l > m1l then
+          begin 
             dyn_ifc' c  pc (R hl' hr)
+          end
+
         end
-      | false, true ->
-        cut (High? lr);
+      | false, true -> 
         let or = interpret_com hr body High in
         if (Some? or) then
         begin
@@ -385,18 +592,22 @@ let rec dyn_ifc' c pc h  =
           let m0r = interpret_exp' hr v in
           let m1r = interpret_exp' hr' v in
           if m0r > m1r then
+          begin
             dyn_ifc' c  pc (R hl hr')
+          end
         end
-      | false, false -> ())
+      | false, false -> ());
+      dyn_ifc_while e body v pc h
   end
   else
   begin
     high_pc c hl pc;
     high_pc c hr pc
   end
-  
-(*
+
 #reset-options    
+
+
 val dyn_ifc : (c:com) -> (env:label_fun) -> (pc:label) ->
     (h:(rel heap)) ->
     Lemma
@@ -408,5 +619,6 @@ val dyn_ifc : (c:com) -> (env:label_fun) -> (pc:label) ->
         (Some?.v r1) (Some?.v r2))
       (interpret_com (R?.l h) c pc)
       (interpret_com (R?.r h) c pc)))
-let dyn_ifc c env pc h = dyn_ifc' c  pc h; high_pc c (R?.l h) pc
-*)
+let dyn_ifc c env pc h = 
+  dyn_ifc' c pc h; 
+  high_pc c (R?.l h) pc
